compiler/backend/presLangScript.sml
@@ -210,6 +210,21 @@ Definition test_to_display_def:
   test_to_display (AltCompare cmp) = Item NONE (strlit "AltCompare") [opb_to_display cmp]
 End
 
+Definition arith_to_display_def:
+  arith_to_display Add = empty_item (strlit "Add") ∧
+  arith_to_display Sub = empty_item (strlit "Sub") ∧
+  arith_to_display Mul = empty_item (strlit "Mul") ∧
+  arith_to_display Div = empty_item (strlit "Div") ∧
+  arith_to_display Mod = empty_item (strlit "Mod") ∧
+  arith_to_display And = empty_item (strlit "And") ∧
+  arith_to_display Xor = empty_item (strlit "Xor") ∧
+  arith_to_display Or  = empty_item (strlit "Or") ∧
+  arith_to_display Neg = empty_item (strlit "Neg") ∧
+  arith_to_display Not = empty_item (strlit "Not") ∧
+  arith_to_display Sqrt = empty_item (strlit "Sqrt") ∧
+  arith_to_display FMA = empty_item (strlit "FMA")
+End
+
 Definition prim_type_to_display_def:
   prim_type_to_display BoolT = empty_item (strlit "BoolT") ∧
   prim_type_to_display IntT = empty_item (strlit "IntT") ∧
@@ -231,6 +246,12 @@ Definition op_to_display_def:
                             [word_size_to_display ws;
                              shift_to_display sh;
                              num_to_display num]
+  | Arith a ty => Item NONE (strlit "Arith")
+                         [arith_to_display a;
+                          prim_type_to_display ty]
+  | FromTo ty1 ty2 => Item NONE (strlit "FromTo")
+                         [prim_type_to_display ty1;
+                          prim_type_to_display ty2]
   | Test test ty => Item NONE (strlit "Test")
                          [test_to_display test;
                           prim_type_to_display ty]
@@ -460,6 +481,12 @@ Definition flat_op_to_display_def:
       word_size_to_display ws;
       shift_to_display sh;
       num_to_display num]
+    | Arith a ty => Item NONE (strlit "Arith")
+                         [arith_to_display a;
+                          prim_type_to_display ty]
+    | FromTo ty1 ty2 => Item NONE (strlit "FromTo")
+                             [prim_type_to_display ty1;
+                              prim_type_to_display ty2]
     | Test test ty => Item NONE (strlit "Test")
                            [test_to_display test;
                             prim_type_to_display ty]
