compiler/backend/proofs/source_to_flatProofScript.sml
@@ -1027,6 +1027,12 @@ Proof
       every_case_tac >>
       full_simp_tac(srw_ss())[] >>
       metis_tac [Boolv_11, do_eq, eq_result_11, eq_result_distinct, v_rel_lems])
+  >~ [‘Arith a ty’] >- (
+      gvs [oneline semanticPrimitivesTheory.do_app_def,AllCaseEqs()]
+      \\ gvs [oneline flatSemTheory.do_app_def,AllCaseEqs()])
+  >~ [‘FromTo ty1 ty2’] >- (
+      gvs [oneline semanticPrimitivesTheory.do_app_def,AllCaseEqs()]
+      \\ gvs [oneline flatSemTheory.do_app_def,AllCaseEqs()])
   >~ [‘Test test ty’] >- (
       gvs [oneline semanticPrimitivesTheory.do_app_def,AllCaseEqs()]
       \\ gvs [oneline flatSemTheory.do_app_def,AllCaseEqs()]
