compiler/inference/inferScript.sml
@@ -609,6 +609,10 @@ Definition op_to_string_def:
   (op_to_string (FpFromWord) = (implode "FpFromWord", 1)) /\
   (op_to_string (Shift _ _ _) = (implode "Shift", 1)) ∧
   (op_to_string Equality = (implode "Equality", 2)) ∧
+  (op_to_string (Arith a ty) =
+     (implode "Arith",
+      dtcase supported_arith a ty of SOME n => (n:num) | NONE => 0n)) ∧
+  (op_to_string (FromTo _ _) = (implode "FromTo", 1)) ∧
   (op_to_string (Test _ _) = (implode "Test", 2)) ∧
   (op_to_string Opapp = (implode "Opapp", 2)) ∧
   (op_to_string Opassign = (implode "Opassign", 2)) ∧
@@ -674,6 +678,13 @@ op_simple_constraints op =
    | Opn _ => (T, [Tem Tint_num; Tem Tint_num], Tem Tint_num)
    | Opb _ => (T, [Tem Tint_num; Tem Tint_num], Tem Tbool_num)
    | Opw wz opw => (T, [Tem (word_tc wz); Tem (word_tc wz)], Tem (word_tc wz))
+   | Arith a ty => (dtcase supported_arith a ty of
+                    | NONE => (F, [], Tem Tbool_num)
+                    | SOME arity =>
+                       (T, REPLICATE arity (Tem (t_num_of ty)), Tem (t_num_of ty)))
+   | FromTo ty1 ty2 => (supported_conversion ty1 ty2,
+                        [Tem (t_num_of ty1)],
+                        Tem (t_num_of ty2))
    | Test test ty => (supported_test test ty,
                       [Tem (t_num_of ty); Tem (t_num_of ty)],
                       Tem Tbool_num)
@@ -807,6 +818,8 @@ constrain_op l op ts s =
    | (Eval, _) => failwith l (implode "Unsafe ops do not have a type") s
    | (Env_id, _) => failwith l (implode "Unsafe ops do not have a type") s
    | (ThunkOp _, _) => failwith l (implode "Thunk ops do not have a type") s
+   | (Arith _ _, _) => failwith l (implode "Type mismatch") s
+   | (FromTo _ _, _) => failwith l (implode "Type mismatch") s
    | (Test _ _, _) => failwith l (implode "Type mismatch") s
    | _ => failwith l (op_n_args_msg op (LENGTH ts)) s
 End
